tyepchecked new chacha20 code

examples/low-level/crypto/Crypto.Symmetric.Chacha20.fst
@@ -7,11 +7,11 @@ open FStar.Buffer
 open FStar.Int.Cast
 open FStar.UInt32
 
+
 let u32 = FStar.UInt32.t
 let uint8_p = buffer FStar.UInt8.t
 
 type chacha_ctx = b:Buffer.buffer u32{length b = 16}
-
 
 val lemma_max_uint32: n:nat -> 
   Lemma (requires (n = 32))
@@ -47,36 +47,12 @@ let store32_le (k:uint8_p) (x:u32) : Stack unit
     k.(3ul) <- uint32_to_uint8 (x >>^ 24ul)
 
 
-val quarter_round:
-  m:chacha_ctx ->
-  a:u32{FStar.UInt32.v a < 16} ->
-  b:u32{FStar.UInt32.v b<16} ->
-  c:u32{FStar.UInt32.v c<16} ->
-  d:u32{FStar.UInt32.v d<16} ->
-  Stack unit
-    (requires (fun h -> live h m))
-    (ensures (fun h0 _ h1 -> live h1 m /\ modifies_1 m h0 h1))
-let quarter_round m a b c d =
-  let ma = m.(a) in let mb = m.(b) in m.(a) <- (ma +%^ mb);
-  let md = m.(d) in let ma = m.(a) in m.(d) <- (md ^^ ma);
-  let md = m.(d) in                   m.(d) <- (md <<< 16ul);
-  let mc = m.(c) in let md = m.(d) in m.(c) <- (mc +%^ md);
-  let mb = m.(b) in let mc = m.(c) in m.(b) <- (mb ^^ mc);
-  let mb = m.(b) in                   m.(b) <- (mb <<< 12ul);
-  let ma = m.(a) in let mb = m.(b) in m.(a) <- (ma +%^ mb);
-  let md = m.(d) in let ma = m.(a) in m.(d) <- (md ^^ ma);
-  let md = m.(d) in                   m.(d) <- (md <<< 8ul);
-  let mc = m.(c) in let md = m.(d) in m.(c) <- (mc +%^ md);
-  let mb = m.(b) in let mc = m.(c) in m.(b) <- (mb ^^ mc);
-  let mb = m.(b) in                   m.(b) <- (mb <<< 7ul)
-
-
 val chacha_keysetup:
   ctx:chacha_ctx ->
-  k:uint8_p ->
+  k:uint8_p{length k = 32 /\ disjoint ctx k} ->
   Stack unit
-    (requires (fun _ -> True))
-    (ensures  (fun _ _ _ -> True))
+    (requires (fun h -> live h ctx /\ live h k))
+    (ensures  (fun h0 _ h1 -> live h1 ctx /\ modifies_1 ctx h0 h1))
 let chacha_keysetup ctx k =
     ctx.(0ul)  <- (0x61707865ul);
     ctx.(1ul)  <- (0x3320646eul);
@@ -92,27 +68,13 @@ let chacha_keysetup ctx k =
     ctx.(11ul) <- load32_le(offset k 28ul)
 
 
-val chacha_ivsetup:
-  ctx:chacha_ctx ->
-  k:uint8_p ->
-  counter:uint8_p ->
-  Stack unit
-    (requires (fun _ -> True))
-    (ensures  (fun _ _ _ -> True))
-let chacha_ivsetup ctx iv counter =
-    ctx.(12ul) <- load32_le(counter);
-    ctx.(13ul) <- load32_le(offset counter 4ul);
-    ctx.(14ul) <- load32_le(iv);
-    ctx.(15ul) <- load32_le(offset iv 4ul)
-
-
 val chacha_ietf_ivsetup:
   ctx:chacha_ctx ->
-  k:uint8_p ->
+  k:uint8_p{length k = 32 /\ disjoint ctx k} ->
   counter:u32 ->
   Stack unit
-    (requires (fun _ -> True))
-    (ensures  (fun _ _ _ -> True))
+    (requires (fun h -> live h ctx /\ live h k))
+    (ensures  (fun h0 _ h1 -> live h1 ctx /\ modifies_1 ctx h0 h1))
 let chacha_ietf_ivsetup ctx iv counter =
     ctx.(12ul) <- counter;
     ctx.(13ul) <- load32_le(iv);
@@ -120,13 +82,15 @@ let chacha_ietf_ivsetup ctx iv counter =
     ctx.(15ul) <- load32_le(offset iv 8ul)
 
 
+#reset-options "--initial_fuel 0 --max_fuel 0 --z3timeout 100"
+
 val chacha_encrypt_bytes_core:
   ctx:chacha_ctx ->
-  m:uint8_p ->
-  c:uint8_p ->
+  m:uint8_p{length m >= 64} ->
+  c:uint8_p{length c >= 64 /\ disjoint ctx c} ->
   Stack unit
-    (requires (fun _ -> True))
-    (ensures  (fun _ _ _ -> True))
+    (requires (fun h -> live h ctx /\ live h c /\ live h m))
+    (ensures  (fun h0 _ h1 -> modifies_1 c h0 h1 /\ live h1 c))
 let chacha_encrypt_bytes_core ctx m c =
   let j0 = ctx.(0ul) in
   let j1 = ctx.(1ul) in
@@ -144,101 +108,6 @@ let chacha_encrypt_bytes_core ctx m c =
   let j13 = ctx.(13ul) in
   let j14 = ctx.(14ul) in
   let j15 = ctx.(15ul) in
-
-  (* let x = Buffer.sub ctx 16ul 16ul in *)
-  (* let ctx = Buffer.sub ctx 0ul 16ul in *)
-  (* blit ctx 0ul x 0ul 16ul; *)
-
-  (* quarter_round x 0ul 4ul 8ul 12ul; *)
-  (* quarter_round x 1ul 5ul 9ul 13ul; *)
-  (* quarter_round x 2ul 6ul 10ul 14ul; *)
-  (* quarter_round x 3ul 7ul 11ul 15ul; *)
-  (* quarter_round x 0ul 5ul 10ul 15ul; *)
-  (* quarter_round x 1ul 6ul 11ul 12ul; *)
-  (* quarter_round x 2ul 7ul 8ul 13ul; *)
-  (* quarter_round x 3ul 4ul 9ul 14ul;   *)
-
-  (* quarter_round x 0ul 4ul 8ul 12ul; *)
-  (* quarter_round x 1ul 5ul 9ul 13ul; *)
-  (* quarter_round x 2ul 6ul 10ul 14ul; *)
-  (* quarter_round x 3ul 7ul 11ul 15ul; *)
-  (* quarter_round x 0ul 5ul 10ul 15ul; *)
-  (* quarter_round x 1ul 6ul 11ul 12ul; *)
-  (* quarter_round x 2ul 7ul 8ul 13ul; *)
-  (* quarter_round x 3ul 4ul 9ul 14ul;   *)
-
-  (* quarter_round x 0ul 4ul 8ul 12ul; *)
-  (* quarter_round x 1ul 5ul 9ul 13ul; *)
-  (* quarter_round x 2ul 6ul 10ul 14ul; *)
-  (* quarter_round x 3ul 7ul 11ul 15ul; *)
-  (* quarter_round x 0ul 5ul 10ul 15ul; *)
-  (* quarter_round x 1ul 6ul 11ul 12ul; *)
-  (* quarter_round x 2ul 7ul 8ul 13ul; *)
-  (* quarter_round x 3ul 4ul 9ul 14ul;   *)
-
-  (* quarter_round x 0ul 4ul 8ul 12ul; *)
-  (* quarter_round x 1ul 5ul 9ul 13ul; *)
-  (* quarter_round x 2ul 6ul 10ul 14ul; *)
-  (* quarter_round x 3ul 7ul 11ul 15ul; *)
-  (* quarter_round x 0ul 5ul 10ul 15ul; *)
-  (* quarter_round x 1ul 6ul 11ul 12ul; *)
-  (* quarter_round x 2ul 7ul 8ul 13ul; *)
-  (* quarter_round x 3ul 4ul 9ul 14ul;   *)
-
-  (* quarter_round x 0ul 4ul 8ul 12ul; *)
-  (* quarter_round x 1ul 5ul 9ul 13ul; *)
-  (* quarter_round x 2ul 6ul 10ul 14ul; *)
-  (* quarter_round x 3ul 7ul 11ul 15ul; *)
-  (* quarter_round x 0ul 5ul 10ul 15ul; *)
-  (* quarter_round x 1ul 6ul 11ul 12ul; *)
-  (* quarter_round x 2ul 7ul 8ul 13ul; *)
-  (* quarter_round x 3ul 4ul 9ul 14ul;   *)
-
-  (* quarter_round x 0ul 4ul 8ul 12ul; *)
-  (* quarter_round x 1ul 5ul 9ul 13ul; *)
-  (* quarter_round x 2ul 6ul 10ul 14ul; *)
-  (* quarter_round x 3ul 7ul 11ul 15ul; *)
-  (* quarter_round x 0ul 5ul 10ul 15ul; *)
-  (* quarter_round x 1ul 6ul 11ul 12ul; *)
-  (* quarter_round x 2ul 7ul 8ul 13ul; *)
-  (* quarter_round x 3ul 4ul 9ul 14ul;   *)
-
-  (* quarter_round x 0ul 4ul 8ul 12ul; *)
-  (* quarter_round x 1ul 5ul 9ul 13ul; *)
-  (* quarter_round x 2ul 6ul 10ul 14ul; *)
-  (* quarter_round x 3ul 7ul 11ul 15ul; *)
-  (* quarter_round x 0ul 5ul 10ul 15ul; *)
-  (* quarter_round x 1ul 6ul 11ul 12ul; *)
-  (* quarter_round x 2ul 7ul 8ul 13ul; *)
-  (* quarter_round x 3ul 4ul 9ul 14ul;   *)
-
-  (* quarter_round x 0ul 4ul 8ul 12ul; *)
-  (* quarter_round x 1ul 5ul 9ul 13ul; *)
-  (* quarter_round x 2ul 6ul 10ul 14ul; *)
-  (* quarter_round x 3ul 7ul 11ul 15ul; *)
-  (* quarter_round x 0ul 5ul 10ul 15ul; *)
-  (* quarter_round x 1ul 6ul 11ul 12ul; *)
-  (* quarter_round x 2ul 7ul 8ul 13ul; *)
-  (* quarter_round x 3ul 4ul 9ul 14ul;   *)
-
-  (* quarter_round x 0ul 4ul 8ul 12ul; *)
-  (* quarter_round x 1ul 5ul 9ul 13ul; *)
-  (* quarter_round x 2ul 6ul 10ul 14ul; *)
-  (* quarter_round x 3ul 7ul 11ul 15ul; *)
-  (* quarter_round x 0ul 5ul 10ul 15ul; *)
-  (* quarter_round x 1ul 6ul 11ul 12ul; *)
-  (* quarter_round x 2ul 7ul 8ul 13ul; *)
-  (* quarter_round x 3ul 4ul 9ul 14ul;   *)
-
-  (* quarter_round x 0ul 4ul 8ul 12ul; *)
-  (* quarter_round x 1ul 5ul 9ul 13ul; *)
-  (* quarter_round x 2ul 6ul 10ul 14ul; *)
-  (* quarter_round x 3ul 7ul 11ul 15ul; *)
-  (* quarter_round x 0ul 5ul 10ul 15ul; *)
-  (* quarter_round x 1ul 6ul 11ul 12ul; *)
-  (* quarter_round x 2ul 7ul 8ul 13ul; *)
-  (* quarter_round x 3ul 4ul 9ul 14ul;   *)
-
   let x0 = j0 in
   let x1 = j1 in
   let x2 = j2 in
@@ -255,7 +124,6 @@ let chacha_encrypt_bytes_core ctx m c =
   let x13 = j13 in
   let x14 = j14 in
   let x15 = j15 in
-
   let x0 = x0 +%^ x4 in
   let x12 = x12 ^^ x0 in
   let x12 = x12 <<< 16ul in
@@ -268,7 +136,6 @@ let chacha_encrypt_bytes_core ctx m c =
   let x8 = x8 +%^ x12 in
   let x4 = x4 ^^ x8 in
   let x4 = x4 <<< 7ul in
-
   let x1 = x1 +%^ x5 in
   let x13 = x13 ^^ x1 in
   let x13 = x13 <<< 16ul in
@@ -281,7 +148,6 @@ let chacha_encrypt_bytes_core ctx m c =
   let x9 = x9 +%^ x13 in
   let x5 = x5 ^^ x9 in
   let x5 = x5 <<< 7ul in
-
   let x2 = x2 +%^ x6 in
   let x14 = x14 ^^ x2 in
   let x14 = x14 <<< 16ul in
@@ -294,7 +160,6 @@ let chacha_encrypt_bytes_core ctx m c =
   let x10 = x10 +%^ x14 in
   let x6 = x6 ^^ x10 in
   let x6 = x6 <<< 7ul in
-
   let x3 = x3 +%^ x7 in
   let x15 = x15 ^^ x3 in
   let x15 = x15 <<< 16ul in
@@ -307,7 +172,6 @@ let chacha_encrypt_bytes_core ctx m c =
   let x11 = x11 +%^ x15 in
   let x7 = x7 ^^ x11 in
   let x7 = x7 <<< 7ul in
-
   let x0 = x0 +%^ x5 in
   let x15 = x15 ^^ x0 in
   let x15 = x15 <<< 16ul in
@@ -320,7 +184,6 @@ let chacha_encrypt_bytes_core ctx m c =
   let x10 = x10 +%^ x15 in
   let x5 = x5 ^^ x10 in
   let x5 = x5 <<< 7ul in
-
   let x1 = x1 +%^ x6 in
   let x12 = x12 ^^ x1 in
   let x12 = x12 <<< 16ul in
@@ -333,7 +196,6 @@ let chacha_encrypt_bytes_core ctx m c =
   let x11 = x11 +%^ x12 in
   let x6 = x6 ^^ x11 in
   let x6 = x6 <<< 7ul in
-
   let x2 = x2 +%^ x7 in
   let x13 = x13 ^^ x2 in
   let x13 = x13 <<< 16ul in
@@ -346,7 +208,6 @@ let chacha_encrypt_bytes_core ctx m c =
   let x8 = x8 +%^ x13 in
   let x7 = x7 ^^ x8 in
   let x7 = x7 <<< 7ul in
-
   let x3 = x3 +%^ x4 in
   let x14 = x14 ^^ x3 in
   let x14 = x14 <<< 16ul in
@@ -359,9 +220,7 @@ let chacha_encrypt_bytes_core ctx m c =
   let x9 = x9 +%^ x14 in
   let x4 = x4 ^^ x9 in
   let x4 = x4 <<< 7ul in
-
   (* 1 *)
-
   let x0 = x0 +%^ x4 in
   let x12 = x12 ^^ x0 in
   let x12 = x12 <<< 16ul in
@@ -374,7 +233,6 @@ let chacha_encrypt_bytes_core ctx m c =
   let x8 = x8 +%^ x12 in
   let x4 = x4 ^^ x8 in
   let x4 = x4 <<< 7ul in
-
   let x1 = x1 +%^ x5 in
   let x13 = x13 ^^ x1 in
   let x13 = x13 <<< 16ul in
@@ -387,7 +245,6 @@ let chacha_encrypt_bytes_core ctx m c =
   let x9 = x9 +%^ x13 in
   let x5 = x5 ^^ x9 in
   let x5 = x5 <<< 7ul in
-
   let x2 = x2 +%^ x6 in
   let x14 = x14 ^^ x2 in
   let x14 = x14 <<< 16ul in
@@ -400,7 +257,6 @@ let chacha_encrypt_bytes_core ctx m c =
   let x10 = x10 +%^ x14 in
   let x6 = x6 ^^ x10 in
   let x6 = x6 <<< 7ul in
-
   let x3 = x3 +%^ x7 in
   let x15 = x15 ^^ x3 in
   let x15 = x15 <<< 16ul in
@@ -413,7 +269,6 @@ let chacha_encrypt_bytes_core ctx m c =
   let x11 = x11 +%^ x15 in
   let x7 = x7 ^^ x11 in
   let x7 = x7 <<< 7ul in
-
   let x0 = x0 +%^ x5 in
   let x15 = x15 ^^ x0 in
   let x15 = x15 <<< 16ul in
@@ -426,7 +281,6 @@ let chacha_encrypt_bytes_core ctx m c =
   let x10 = x10 +%^ x15 in
   let x5 = x5 ^^ x10 in
   let x5 = x5 <<< 7ul in
-
   let x1 = x1 +%^ x6 in
   let x12 = x12 ^^ x1 in
   let x12 = x12 <<< 16ul in
@@ -439,7 +293,6 @@ let chacha_encrypt_bytes_core ctx m c =
   let x11 = x11 +%^ x12 in
   let x6 = x6 ^^ x11 in
   let x6 = x6 <<< 7ul in
-
   let x2 = x2 +%^ x7 in
   let x13 = x13 ^^ x2 in
   let x13 = x13 <<< 16ul in
@@ -452,7 +305,6 @@ let chacha_encrypt_bytes_core ctx m c =
   let x8 = x8 +%^ x13 in
   let x7 = x7 ^^ x8 in
   let x7 = x7 <<< 7ul in
-
   let x3 = x3 +%^ x4 in
   let x14 = x14 ^^ x3 in
   let x14 = x14 <<< 16ul in
@@ -465,9 +317,7 @@ let chacha_encrypt_bytes_core ctx m c =
   let x9 = x9 +%^ x14 in
   let x4 = x4 ^^ x9 in
   let x4 = x4 <<< 7ul in
-
   (* 2 *)
-
   let x0 = x0 +%^ x4 in
   let x12 = x12 ^^ x0 in
   let x12 = x12 <<< 16ul in
@@ -480,7 +330,6 @@ let chacha_encrypt_bytes_core ctx m c =
   let x8 = x8 +%^ x12 in
   let x4 = x4 ^^ x8 in
   let x4 = x4 <<< 7ul in
-
   let x1 = x1 +%^ x5 in
   let x13 = x13 ^^ x1 in
   let x13 = x13 <<< 16ul in
@@ -493,7 +342,6 @@ let chacha_encrypt_bytes_core ctx m c =
   let x9 = x9 +%^ x13 in
   let x5 = x5 ^^ x9 in
   let x5 = x5 <<< 7ul in
-
   let x2 = x2 +%^ x6 in
   let x14 = x14 ^^ x2 in
   let x14 = x14 <<< 16ul in
@@ -506,7 +354,6 @@ let chacha_encrypt_bytes_core ctx m c =
   let x10 = x10 +%^ x14 in
   let x6 = x6 ^^ x10 in
   let x6 = x6 <<< 7ul in
-
   let x3 = x3 +%^ x7 in
   let x15 = x15 ^^ x3 in
   let x15 = x15 <<< 16ul in
@@ -519,7 +366,6 @@ let chacha_encrypt_bytes_core ctx m c =
   let x11 = x11 +%^ x15 in
   let x7 = x7 ^^ x11 in
   let x7 = x7 <<< 7ul in
-
   let x0 = x0 +%^ x5 in
   let x15 = x15 ^^ x0 in
   let x15 = x15 <<< 16ul in
@@ -532,7 +378,6 @@ let chacha_encrypt_bytes_core ctx m c =
   let x10 = x10 +%^ x15 in
   let x5 = x5 ^^ x10 in
   let x5 = x5 <<< 7ul in
-
   let x1 = x1 +%^ x6 in
   let x12 = x12 ^^ x1 in
   let x12 = x12 <<< 16ul in
@@ -545,7 +390,6 @@ let chacha_encrypt_bytes_core ctx m c =
   let x11 = x11 +%^ x12 in
   let x6 = x6 ^^ x11 in
   let x6 = x6 <<< 7ul in
-
   let x2 = x2 +%^ x7 in
   let x13 = x13 ^^ x2 in
   let x13 = x13 <<< 16ul in
@@ -558,7 +402,6 @@ let chacha_encrypt_bytes_core ctx m c =
   let x8 = x8 +%^ x13 in
   let x7 = x7 ^^ x8 in
   let x7 = x7 <<< 7ul in
-
   let x3 = x3 +%^ x4 in
   let x14 = x14 ^^ x3 in
   let x14 = x14 <<< 16ul in
@@ -571,9 +414,7 @@ let chacha_encrypt_bytes_core ctx m c =
   let x9 = x9 +%^ x14 in
   let x4 = x4 ^^ x9 in
   let x4 = x4 <<< 7ul in
-
   (* 3 *)
-
   let x0 = x0 +%^ x4 in
   let x12 = x12 ^^ x0 in
   let x12 = x12 <<< 16ul in
@@ -586,7 +427,6 @@ let chacha_encrypt_bytes_core ctx m c =
   let x8 = x8 +%^ x12 in
   let x4 = x4 ^^ x8 in
   let x4 = x4 <<< 7ul in
-
   let x1 = x1 +%^ x5 in
   let x13 = x13 ^^ x1 in
   let x13 = x13 <<< 16ul in
@@ -599,7 +439,6 @@ let chacha_encrypt_bytes_core ctx m c =
   let x9 = x9 +%^ x13 in
   let x5 = x5 ^^ x9 in
   let x5 = x5 <<< 7ul in
-
   let x2 = x2 +%^ x6 in
   let x14 = x14 ^^ x2 in
   let x14 = x14 <<< 16ul in
@@ -612,7 +451,6 @@ let chacha_encrypt_bytes_core ctx m c =
   let x10 = x10 +%^ x14 in
   let x6 = x6 ^^ x10 in
   let x6 = x6 <<< 7ul in
-
   let x3 = x3 +%^ x7 in
   let x15 = x15 ^^ x3 in
   let x15 = x15 <<< 16ul in
@@ -625,7 +463,6 @@ let chacha_encrypt_bytes_core ctx m c =
   let x11 = x11 +%^ x15 in
   let x7 = x7 ^^ x11 in
   let x7 = x7 <<< 7ul in
-
   let x0 = x0 +%^ x5 in
   let x15 = x15 ^^ x0 in
   let x15 = x15 <<< 16ul in
@@ -638,7 +475,6 @@ let chacha_encrypt_bytes_core ctx m c =
   let x10 = x10 +%^ x15 in
   let x5 = x5 ^^ x10 in
   let x5 = x5 <<< 7ul in
-
   let x1 = x1 +%^ x6 in
   let x12 = x12 ^^ x1 in
   let x12 = x12 <<< 16ul in
@@ -651,7 +487,6 @@ let chacha_encrypt_bytes_core ctx m c =
   let x11 = x11 +%^ x12 in
   let x6 = x6 ^^ x11 in
   let x6 = x6 <<< 7ul in
-
   let x2 = x2 +%^ x7 in
   let x13 = x13 ^^ x2 in
   let x13 = x13 <<< 16ul in
@@ -664,7 +499,6 @@ let chacha_encrypt_bytes_core ctx m c =
   let x8 = x8 +%^ x13 in
   let x7 = x7 ^^ x8 in
   let x7 = x7 <<< 7ul in
-
   let x3 = x3 +%^ x4 in
   let x14 = x14 ^^ x3 in
   let x14 = x14 <<< 16ul in
@@ -677,9 +511,7 @@ let chacha_encrypt_bytes_core ctx m c =
   let x9 = x9 +%^ x14 in
   let x4 = x4 ^^ x9 in
   let x4 = x4 <<< 7ul in
-
   (* 4 *)
-
   let x0 = x0 +%^ x4 in
   let x12 = x12 ^^ x0 in
   let x12 = x12 <<< 16ul in
@@ -692,7 +524,6 @@ let chacha_encrypt_bytes_core ctx m c =
   let x8 = x8 +%^ x12 in
   let x4 = x4 ^^ x8 in
   let x4 = x4 <<< 7ul in
-
   let x1 = x1 +%^ x5 in
   let x13 = x13 ^^ x1 in
   let x13 = x13 <<< 16ul in
@@ -705,7 +536,6 @@ let chacha_encrypt_bytes_core ctx m c =
   let x9 = x9 +%^ x13 in
   let x5 = x5 ^^ x9 in
   let x5 = x5 <<< 7ul in
-
   let x2 = x2 +%^ x6 in
   let x14 = x14 ^^ x2 in
   let x14 = x14 <<< 16ul in
@@ -718,7 +548,6 @@ let chacha_encrypt_bytes_core ctx m c =
   let x10 = x10 +%^ x14 in
   let x6 = x6 ^^ x10 in
   let x6 = x6 <<< 7ul in
-
   let x3 = x3 +%^ x7 in
   let x15 = x15 ^^ x3 in
   let x15 = x15 <<< 16ul in
@@ -731,7 +560,6 @@ let chacha_encrypt_bytes_core ctx m c =
   let x11 = x11 +%^ x15 in
   let x7 = x7 ^^ x11 in
   let x7 = x7 <<< 7ul in
-
   let x0 = x0 +%^ x5 in
   let x15 = x15 ^^ x0 in
   let x15 = x15 <<< 16ul in
@@ -744,7 +572,6 @@ let chacha_encrypt_bytes_core ctx m c =
   let x10 = x10 +%^ x15 in
   let x5 = x5 ^^ x10 in
   let x5 = x5 <<< 7ul in
-
   let x1 = x1 +%^ x6 in
   let x12 = x12 ^^ x1 in
   let x12 = x12 <<< 16ul in
@@ -757,7 +584,6 @@ let chacha_encrypt_bytes_core ctx m c =
   let x11 = x11 +%^ x12 in
   let x6 = x6 ^^ x11 in
   let x6 = x6 <<< 7ul in
-
   let x2 = x2 +%^ x7 in
   let x13 = x13 ^^ x2 in
   let x13 = x13 <<< 16ul in
@@ -770,7 +596,6 @@ let chacha_encrypt_bytes_core ctx m c =
   let x8 = x8 +%^ x13 in
   let x7 = x7 ^^ x8 in
   let x7 = x7 <<< 7ul in
-
   let x3 = x3 +%^ x4 in
   let x14 = x14 ^^ x3 in
   let x14 = x14 <<< 16ul in
@@ -783,9 +608,7 @@ let chacha_encrypt_bytes_core ctx m c =
   let x9 = x9 +%^ x14 in
   let x4 = x4 ^^ x9 in
   let x4 = x4 <<< 7ul in
-
   (* 5 *)
-
   let x0 = x0 +%^ x4 in
   let x12 = x12 ^^ x0 in
   let x12 = x12 <<< 16ul in
@@ -798,7 +621,6 @@ let chacha_encrypt_bytes_core ctx m c =
   let x8 = x8 +%^ x12 in
   let x4 = x4 ^^ x8 in
   let x4 = x4 <<< 7ul in
-
   let x1 = x1 +%^ x5 in
   let x13 = x13 ^^ x1 in
   let x13 = x13 <<< 16ul in
@@ -811,7 +633,6 @@ let chacha_encrypt_bytes_core ctx m c =
   let x9 = x9 +%^ x13 in
   let x5 = x5 ^^ x9 in
   let x5 = x5 <<< 7ul in
-
   let x2 = x2 +%^ x6 in
   let x14 = x14 ^^ x2 in
   let x14 = x14 <<< 16ul in
@@ -824,7 +645,6 @@ let chacha_encrypt_bytes_core ctx m c =
   let x10 = x10 +%^ x14 in
   let x6 = x6 ^^ x10 in
   let x6 = x6 <<< 7ul in
-
   let x3 = x3 +%^ x7 in
   let x15 = x15 ^^ x3 in
   let x15 = x15 <<< 16ul in
@@ -837,7 +657,6 @@ let chacha_encrypt_bytes_core ctx m c =
   let x11 = x11 +%^ x15 in
   let x7 = x7 ^^ x11 in
   let x7 = x7 <<< 7ul in
-
   let x0 = x0 +%^ x5 in
   let x15 = x15 ^^ x0 in
   let x15 = x15 <<< 16ul in
@@ -850,7 +669,6 @@ let chacha_encrypt_bytes_core ctx m c =
   let x10 = x10 +%^ x15 in
   let x5 = x5 ^^ x10 in
   let x5 = x5 <<< 7ul in
-
   let x1 = x1 +%^ x6 in
   let x12 = x12 ^^ x1 in
   let x12 = x12 <<< 16ul in
@@ -863,7 +681,6 @@ let chacha_encrypt_bytes_core ctx m c =
   let x11 = x11 +%^ x12 in
   let x6 = x6 ^^ x11 in
   let x6 = x6 <<< 7ul in
-
   let x2 = x2 +%^ x7 in
   let x13 = x13 ^^ x2 in
   let x13 = x13 <<< 16ul in
@@ -876,7 +693,6 @@ let chacha_encrypt_bytes_core ctx m c =
   let x8 = x8 +%^ x13 in
   let x7 = x7 ^^ x8 in
   let x7 = x7 <<< 7ul in
-
   let x3 = x3 +%^ x4 in
   let x14 = x14 ^^ x3 in
   let x14 = x14 <<< 16ul in
@@ -889,9 +705,7 @@ let chacha_encrypt_bytes_core ctx m c =
   let x9 = x9 +%^ x14 in
   let x4 = x4 ^^ x9 in
   let x4 = x4 <<< 7ul in
-
   (* 6 *)
-
   let x0 = x0 +%^ x4 in
   let x12 = x12 ^^ x0 in
   let x12 = x12 <<< 16ul in
@@ -904,7 +718,6 @@ let chacha_encrypt_bytes_core ctx m c =
   let x8 = x8 +%^ x12 in
   let x4 = x4 ^^ x8 in
   let x4 = x4 <<< 7ul in
-
   let x1 = x1 +%^ x5 in
   let x13 = x13 ^^ x1 in
   let x13 = x13 <<< 16ul in
@@ -917,7 +730,6 @@ let chacha_encrypt_bytes_core ctx m c =
   let x9 = x9 +%^ x13 in
   let x5 = x5 ^^ x9 in
   let x5 = x5 <<< 7ul in
-
   let x2 = x2 +%^ x6 in
   let x14 = x14 ^^ x2 in
   let x14 = x14 <<< 16ul in
@@ -930,7 +742,6 @@ let chacha_encrypt_bytes_core ctx m c =
   let x10 = x10 +%^ x14 in
   let x6 = x6 ^^ x10 in
   let x6 = x6 <<< 7ul in
-
   let x3 = x3 +%^ x7 in
   let x15 = x15 ^^ x3 in
   let x15 = x15 <<< 16ul in
@@ -943,7 +754,6 @@ let chacha_encrypt_bytes_core ctx m c =
   let x11 = x11 +%^ x15 in
   let x7 = x7 ^^ x11 in
   let x7 = x7 <<< 7ul in
-
   let x0 = x0 +%^ x5 in
   let x15 = x15 ^^ x0 in
   let x15 = x15 <<< 16ul in
@@ -956,7 +766,6 @@ let chacha_encrypt_bytes_core ctx m c =
   let x10 = x10 +%^ x15 in
   let x5 = x5 ^^ x10 in
   let x5 = x5 <<< 7ul in
-
   let x1 = x1 +%^ x6 in
   let x12 = x12 ^^ x1 in
   let x12 = x12 <<< 16ul in
@@ -969,7 +778,6 @@ let chacha_encrypt_bytes_core ctx m c =
   let x11 = x11 +%^ x12 in
   let x6 = x6 ^^ x11 in
   let x6 = x6 <<< 7ul in
-
   let x2 = x2 +%^ x7 in
   let x13 = x13 ^^ x2 in
   let x13 = x13 <<< 16ul in
@@ -982,7 +790,6 @@ let chacha_encrypt_bytes_core ctx m c =
   let x8 = x8 +%^ x13 in
   let x7 = x7 ^^ x8 in
   let x7 = x7 <<< 7ul in
-
   let x3 = x3 +%^ x4 in
   let x14 = x14 ^^ x3 in
   let x14 = x14 <<< 16ul in
@@ -995,9 +802,7 @@ let chacha_encrypt_bytes_core ctx m c =
   let x9 = x9 +%^ x14 in
   let x4 = x4 ^^ x9 in
   let x4 = x4 <<< 7ul in
-
   (* 7 *)
-
   let x0 = x0 +%^ x4 in
   let x12 = x12 ^^ x0 in
   let x12 = x12 <<< 16ul in
@@ -1010,7 +815,6 @@ let chacha_encrypt_bytes_core ctx m c =
   let x8 = x8 +%^ x12 in
   let x4 = x4 ^^ x8 in
   let x4 = x4 <<< 7ul in
-
   let x1 = x1 +%^ x5 in
   let x13 = x13 ^^ x1 in
   let x13 = x13 <<< 16ul in
@@ -1023,7 +827,6 @@ let chacha_encrypt_bytes_core ctx m c =
   let x9 = x9 +%^ x13 in
   let x5 = x5 ^^ x9 in
   let x5 = x5 <<< 7ul in
-
   let x2 = x2 +%^ x6 in
   let x14 = x14 ^^ x2 in
   let x14 = x14 <<< 16ul in
@@ -1036,7 +839,6 @@ let chacha_encrypt_bytes_core ctx m c =
   let x10 = x10 +%^ x14 in
   let x6 = x6 ^^ x10 in
   let x6 = x6 <<< 7ul in
-
   let x3 = x3 +%^ x7 in
   let x15 = x15 ^^ x3 in
   let x15 = x15 <<< 16ul in
@@ -1049,7 +851,6 @@ let chacha_encrypt_bytes_core ctx m c =
   let x11 = x11 +%^ x15 in
   let x7 = x7 ^^ x11 in
   let x7 = x7 <<< 7ul in
-
   let x0 = x0 +%^ x5 in
   let x15 = x15 ^^ x0 in
   let x15 = x15 <<< 16ul in
@@ -1062,7 +863,6 @@ let chacha_encrypt_bytes_core ctx m c =
   let x10 = x10 +%^ x15 in
   let x5 = x5 ^^ x10 in
   let x5 = x5 <<< 7ul in
-
   let x1 = x1 +%^ x6 in
   let x12 = x12 ^^ x1 in
   let x12 = x12 <<< 16ul in
@@ -1075,7 +875,6 @@ let chacha_encrypt_bytes_core ctx m c =
   let x11 = x11 +%^ x12 in
   let x6 = x6 ^^ x11 in
   let x6 = x6 <<< 7ul in
-
   let x2 = x2 +%^ x7 in
   let x13 = x13 ^^ x2 in
   let x13 = x13 <<< 16ul in
@@ -1088,7 +887,6 @@ let chacha_encrypt_bytes_core ctx m c =
   let x8 = x8 +%^ x13 in
   let x7 = x7 ^^ x8 in
   let x7 = x7 <<< 7ul in
-
   let x3 = x3 +%^ x4 in
   let x14 = x14 ^^ x3 in
   let x14 = x14 <<< 16ul in
@@ -1101,9 +899,7 @@ let chacha_encrypt_bytes_core ctx m c =
   let x9 = x9 +%^ x14 in
   let x4 = x4 ^^ x9 in
   let x4 = x4 <<< 7ul in
-
   (* 8 *)
-
   let x0 = x0 +%^ x4 in
   let x12 = x12 ^^ x0 in
   let x12 = x12 <<< 16ul in
@@ -1116,7 +912,6 @@ let chacha_encrypt_bytes_core ctx m c =
   let x8 = x8 +%^ x12 in
   let x4 = x4 ^^ x8 in
   let x4 = x4 <<< 7ul in
-
   let x1 = x1 +%^ x5 in
   let x13 = x13 ^^ x1 in
   let x13 = x13 <<< 16ul in
@@ -1129,7 +924,6 @@ let chacha_encrypt_bytes_core ctx m c =
   let x9 = x9 +%^ x13 in
   let x5 = x5 ^^ x9 in
   let x5 = x5 <<< 7ul in
-
   let x2 = x2 +%^ x6 in
   let x14 = x14 ^^ x2 in
   let x14 = x14 <<< 16ul in
@@ -1142,7 +936,6 @@ let chacha_encrypt_bytes_core ctx m c =
   let x10 = x10 +%^ x14 in
   let x6 = x6 ^^ x10 in
   let x6 = x6 <<< 7ul in
-
   let x3 = x3 +%^ x7 in
   let x15 = x15 ^^ x3 in
   let x15 = x15 <<< 16ul in
@@ -1155,7 +948,6 @@ let chacha_encrypt_bytes_core ctx m c =
   let x11 = x11 +%^ x15 in
   let x7 = x7 ^^ x11 in
   let x7 = x7 <<< 7ul in
-
   let x0 = x0 +%^ x5 in
   let x15 = x15 ^^ x0 in
   let x15 = x15 <<< 16ul in
@@ -1168,7 +960,6 @@ let chacha_encrypt_bytes_core ctx m c =
   let x10 = x10 +%^ x15 in
   let x5 = x5 ^^ x10 in
   let x5 = x5 <<< 7ul in
-
   let x1 = x1 +%^ x6 in
   let x12 = x12 ^^ x1 in
   let x12 = x12 <<< 16ul in
@@ -1181,7 +972,6 @@ let chacha_encrypt_bytes_core ctx m c =
   let x11 = x11 +%^ x12 in
   let x6 = x6 ^^ x11 in
   let x6 = x6 <<< 7ul in
-
   let x2 = x2 +%^ x7 in
   let x13 = x13 ^^ x2 in
   let x13 = x13 <<< 16ul in
@@ -1194,7 +984,6 @@ let chacha_encrypt_bytes_core ctx m c =
   let x8 = x8 +%^ x13 in
   let x7 = x7 ^^ x8 in
   let x7 = x7 <<< 7ul in
-
   let x3 = x3 +%^ x4 in
   let x14 = x14 ^^ x3 in
   let x14 = x14 <<< 16ul in
@@ -1207,9 +996,7 @@ let chacha_encrypt_bytes_core ctx m c =
   let x9 = x9 +%^ x14 in
   let x4 = x4 ^^ x9 in
   let x4 = x4 <<< 7ul in
-
   (* 9 *)
-
   let x0 = x0 +%^ x4 in
   let x12 = x12 ^^ x0 in
   let x12 = x12 <<< 16ul in
@@ -1222,7 +1009,6 @@ let chacha_encrypt_bytes_core ctx m c =
   let x8 = x8 +%^ x12 in
   let x4 = x4 ^^ x8 in
   let x4 = x4 <<< 7ul in
-
   let x1 = x1 +%^ x5 in
   let x13 = x13 ^^ x1 in
   let x13 = x13 <<< 16ul in
@@ -1235,7 +1021,6 @@ let chacha_encrypt_bytes_core ctx m c =
   let x9 = x9 +%^ x13 in
   let x5 = x5 ^^ x9 in
   let x5 = x5 <<< 7ul in
-
   let x2 = x2 +%^ x6 in
   let x14 = x14 ^^ x2 in
   let x14 = x14 <<< 16ul in
@@ -1248,7 +1033,6 @@ let chacha_encrypt_bytes_core ctx m c =
   let x10 = x10 +%^ x14 in
   let x6 = x6 ^^ x10 in
   let x6 = x6 <<< 7ul in
-
   let x3 = x3 +%^ x7 in
   let x15 = x15 ^^ x3 in
   let x15 = x15 <<< 16ul in
@@ -1261,7 +1045,6 @@ let chacha_encrypt_bytes_core ctx m c =
   let x11 = x11 +%^ x15 in
   let x7 = x7 ^^ x11 in
   let x7 = x7 <<< 7ul in
-
   let x0 = x0 +%^ x5 in
   let x15 = x15 ^^ x0 in
   let x15 = x15 <<< 16ul in
@@ -1274,7 +1057,6 @@ let chacha_encrypt_bytes_core ctx m c =
   let x10 = x10 +%^ x15 in
   let x5 = x5 ^^ x10 in
   let x5 = x5 <<< 7ul in
-
   let x1 = x1 +%^ x6 in
   let x12 = x12 ^^ x1 in
   let x12 = x12 <<< 16ul in
@@ -1287,7 +1069,6 @@ let chacha_encrypt_bytes_core ctx m c =
   let x11 = x11 +%^ x12 in
   let x6 = x6 ^^ x11 in
   let x6 = x6 <<< 7ul in
-
   let x2 = x2 +%^ x7 in
   let x13 = x13 ^^ x2 in
   let x13 = x13 <<< 16ul in
@@ -1300,7 +1081,6 @@ let chacha_encrypt_bytes_core ctx m c =
   let x8 = x8 +%^ x13 in
   let x7 = x7 ^^ x8 in
   let x7 = x7 <<< 7ul in
-
   let x3 = x3 +%^ x4 in
   let x14 = x14 ^^ x3 in
   let x14 = x14 <<< 16ul in
@@ -1313,42 +1093,23 @@ let chacha_encrypt_bytes_core ctx m c =
   let x9 = x9 +%^ x14 in
   let x4 = x4 ^^ x9 in
   let x4 = x4 <<< 7ul in
- 
-  (* (\* 10 *\) *)
-  (* let x0 = x.(0ul) in *)
-  (* let x1 = x.(1ul) in *)
-  (* let x2 = x.(2ul) in *)
-  (* let x3 = x.(3ul) in *)
-  (* let x4 = x.(4ul) in *)
-  (* let x5 = x.(5ul) in *)
-  (* let x6 = x.(6ul) in *)
-  (* let x7 = x.(7ul) in *)
-  (* let x8 = x.(8ul) in *)
-  (* let x9 = x.(9ul) in *)
-  (* let x10 = x.(10ul) in *)
-  (* let x11 = x.(11ul) in *)
-  (* let x12 = x.(12ul) in *)
-  (* let x13 = x.(13ul) in *)
-  (* let x14 = x.(14ul) in *)
-  (* let x15 = x.(15ul) in *)
-
-  let x0 = x0 +^ j0 in
-  let x1 = x1 +^ j1 in
-  let x2 = x2 +^ j2 in
-  let x3 = x3 +^ j3 in
-  let x4 = x4 +^ j4 in
-  let x5 = x5 +^ j5 in
-  let x6 = x6 +^ j6 in
-  let x7 = x7 +^ j7 in
-  let x8 = x8 +^ j8 in
-  let x9 = x9 +^ j9 in
-  let x10 = x10 +^ j10 in
-  let x11 = x11 +^ j11 in
-  let x12 = x12 +^ j12 in
-  let x13 = x13 +^ j13 in
-  let x14 = x14 +^ j14 in
-  let x15 = x15 +^ j15 in
-
+  (* 10 *)
+  let x0 = x0 +%^ j0 in
+  let x1 = x1 +%^ j1 in
+  let x2 = x2 +%^ j2 in
+  let x3 = x3 +%^ j3 in
+  let x4 = x4 +%^ j4 in
+  let x5 = x5 +%^ j5 in
+  let x6 = x6 +%^ j6 in
+  let x7 = x7 +%^ j7 in
+  let x8 = x8 +%^ j8 in
+  let x9 = x9 +%^ j9 in
+  let x10 = x10 +%^ j10 in
+  let x11 = x11 +%^ j11 in
+  let x12 = x12 +%^ j12 in
+  let x13 = x13 +%^ j13 in
+  let x14 = x14 +%^ j14 in
+  let x15 = x15 +%^ j15 in
   let open FStar.Buffer in
   let m0 = load32_le (sub m 0ul 4ul) in
   let m1 = load32_le (sub m 4ul 4ul) in
@@ -1366,7 +1127,6 @@ let chacha_encrypt_bytes_core ctx m c =
   let m13 = load32_le (sub m 52ul 4ul) in
   let m14 = load32_le (sub m 56ul 4ul) in
   let m15 = load32_le (sub m 60ul 4ul) in
-
   let x0 = x0 ^^ m0 in
   let x1 = x1 ^^ m1 in
   let x2 = x2 ^^ m2 in
@@ -1383,7 +1143,6 @@ let chacha_encrypt_bytes_core ctx m c =
   let x13 = x13 ^^ m13 in
   let x14 = x14 ^^ m14 in
   let x15 = x15 ^^ m15 in
-
   store32_le (sub c 0ul 4ul) x0;
   store32_le (sub c 4ul 4ul) x1;
   store32_le (sub c 8ul 4ul) x2;
@@ -1402,295 +1161,68 @@ let chacha_encrypt_bytes_core ctx m c =
   store32_le (sub c 60ul 4ul) x15
 
 
+module U32 = FStar.UInt32
+
 val chacha_encrypt_bytes_loop:
   ctx:chacha_ctx ->
   m:uint8_p ->
-  c:uint8_p ->
-  len:UInt32.t ->
+  c:uint8_p{disjoint ctx c} ->
+  len:U32.t{U32.v len <= length m /\ U32.v len <= length c} ->
   Stack unit
-    (requires (fun _ -> True))
-    (ensures  (fun _ _ _ -> True))
+    (requires (fun h -> live h c /\ live h m /\ live h ctx))
+    (ensures  (fun h0 _ h1 -> live h1 c /\ modifies_2 ctx c h0 h1))
 let rec chacha_encrypt_bytes_loop ctx m c len =
   if FStar.UInt32 (len <^ 64ul) then ()
   else (
     chacha_encrypt_bytes_core ctx m c;
     let ctr = ctx.(12ul) in
-    ctx.(12ul) <- FStar.UInt32 (ctr +^ 1ul);
+    ctx.(12ul) <- FStar.UInt32 (ctr +%^ 1ul);
     chacha_encrypt_bytes_loop ctx (offset m 64ul) (offset c 64ul) (FStar.UInt32 (len -^ 64ul))
   )
 
 
-module U32 = FStar.UInt32
+val chacha_encrypt_bytes_finish:
+  ctx:chacha_ctx ->
+  m:uint8_p ->
+  c:uint8_p{disjoint ctx c} ->
+  len:UInt32.t{U32.v len <= length m /\ U32.v len <= length c /\ U32.v len < 64} ->
+  Stack unit
+    (requires (fun h -> live h c /\ live h m /\ live h ctx))
+    (ensures  (fun h0 _ h1 -> live h1 c /\ modifies_2 ctx c h0 h1))
+let chacha_encrypt_bytes_finish ctx m c len =
+  let hinit = ST.get() in
+  push_frame();
+  let h0 = ST.get() in
+  let tmp = create (0uy) 64ul in
+  let h0' = ST.get() in
+  blit m 0ul tmp 0ul len;
+  let h1 = ST.get() in
+  chacha_encrypt_bytes_core ctx tmp tmp;
+  let h2 = ST.get() in
+  blit tmp 0ul c 0ul len;
+  let h3 = ST.get() in
+  lemma_modifies_2_1'' ctx c h0 h2 h3;
+  pop_frame();
+  let hfin = ST.get() in
+  ()
+
 
 val chacha_encrypt_bytes:
   ctx:chacha_ctx ->
   m:uint8_p ->
-  c:uint8_p ->
-  len:UInt32.t ->
+  c:uint8_p{disjoint ctx c} ->
+  len:UInt32.t{U32.v len <= length m /\ U32.v len <= length c} ->
   Stack unit
-    (requires (fun _ -> True))
-    (ensures  (fun _ _ _ -> True))
+    (requires (fun h -> live h c /\ live h m /\ live h ctx))
+    (ensures  (fun h0 _ h1 -> live h1 c /\ modifies_2 ctx c h0 h1))
 let rec chacha_encrypt_bytes ctx m c len =
-  push_frame();
   chacha_encrypt_bytes_loop ctx m c len;
+  UInt.logand_mask (U32.v len) 6;
+  assert_norm(pow2 6 = 64);
+  Math.Lemmas.euclidean_division_definition (v len) 64;
   let rem = U32 (len &^ 63ul) in // % 64
   let q   = U32 (len >>^ 6ul) in // / 64
   if FStar.UInt32 (rem >=^ 0ul) then (
-    let tmp = create (0uy) 64ul in
     let m = offset m (U32 (len -^ rem)) in
     let c = offset c (U32 (len -^ rem)) in
-    blit m 0ul tmp 0ul rem;
-    chacha_encrypt_bytes_core ctx tmp tmp;
-    blit tmp 0ul c 0ul rem );
-  pop_frame()
-
-
-
-(* // Concrete implementation of CHACHA20 and countermode encryption *)
-(* // Not much point verifying its against a more complex pure specification. *)
-
-(* open FStar.Mul *)
-(* open FStar.Ghost *)
-(* (\*  Machine integers *\) *)
-(* open FStar.UInt8 *)
-(* open FStar.UInt32 *)
-(* open FStar.Int.Cast *)
-(* (\*  Effects and memory layout *\) *)
-(* open FStar.HyperStack *)
-(* (\*  Buffers *\) *)
-(* open FStar.Buffer *)
-(* open Buffer.Utils *)
-
-(* module HH = FStar.HyperHeap *)
-(* module HS = FStar.HyperStack *)
-
-(* type u64 = FStar.UInt64.t *)
-
-
-(* (\*** Chacha 20 ***\) *)
-
-(* inline_for_extraction let keylen   = 32ul *)
-(* inline_for_extraction let blocklen = 64ul  *)
-(* inline_for_extraction let ivlen    = 12ul *)
-
-(* type lbytes l = b:bytes {length b = l} *)
-(* type key   = lbytes (v keylen) *)
-(* type block = lbytes (v blocklen) *)
-(* type iv    = lbytes (v ivlen) *)
-
-(* // internally, blocks are represented as 16 x 4-byte integers *)
-(* private type matrix = m:uint32s{length m = v blocklen / 4} *)
-
-(* private type shuffle =  *)
-(*   m:matrix -> STL unit *)
-(*   (requires (fun h -> live h m)) *)
-(*   (ensures (fun h0 _ h1 -> live h1 m /\ modifies_1 m h0 h1 )) *)
-
-(* (\* lifted by hand for now: *\) *)
-(* private val line: *)
-(*   m:matrix ->  *)
-(*   a:u32{v a < 16} ->  *)
-(*   b:u32{v b < 16} ->  *)
-(*   d:u32{v d < 16} ->  *)
-(*   s:u32{v s <= 32}-> STL unit *)
-(*   (requires (fun h -> live h m)) *)
-(*   (ensures (fun h0 _ h1 -> live h1 m /\ modifies_1 m h0 h1 )) *)
-(* let line m a b d s =  *)
-(*   m.(a) <- m.(a) +%^ m.(b); *)
-(*   m.(d) <-(m.(d) ^^  m.(a)) <<< s *)
-
-(* private val quarter_round: *)
-(*   m:matrix ->  *)
-(*   a:u32{v a < 16} ->  *)
-(*   b:u32{v b < 16} ->  *)
-(*   c:u32{v c < 16} ->  *)
-(*   d:u32{v d < 16} -> STL unit *)
-(*   (requires (fun h -> live h m)) *)
-(*   (ensures (fun h0 _ h1 -> live h1 m /\ modifies_1 m h0 h1 )) *)
-(* let quarter_round m a b c d =  *)
-(* (\* *)
-(*   let line a b d s =  *)
-(*     upd m a (m.(a) +%^ m.(b)); *)
-(*     upd m d((m.(d) ^^  m.(a)) <<< s) in *)
-(* *\)     *)
-(*   line m a b d 16ul; *)
-(*   line m c d b 12ul; *)
-(*   line m a b d  8ul;  *)
-(*   line m c d b  7ul *)
-
-(* private val column_round: shuffle  *)
-(* let column_round m = *)
-(*   quarter_round m 0ul 4ul  8ul 12ul; *)
-(*   quarter_round m 1ul 5ul  9ul 13ul; *)
-(*   quarter_round m 2ul 6ul 10ul 14ul; *)
-(*   quarter_round m 3ul 7ul 11ul 15ul *)
-
-(* private val diagonal_round: shuffle *)
-(* let diagonal_round m = *)
-(*   quarter_round m 0ul 5ul 10ul 15ul; *)
-(*   quarter_round m 1ul 6ul 11ul 12ul; *)
-(*   quarter_round m 2ul 7ul  8ul 13ul; *)
-(*   quarter_round m 3ul 4ul  9ul 14ul *)
-
-(* private val rounds: shuffle  *)
-(* let rounds m = (\* 20 rounds *\) *)
-(*   column_round m; diagonal_round m;  *)
-(*   column_round m; diagonal_round m; *)
-(*   column_round m; diagonal_round m; *)
-(*   column_round m; diagonal_round m; *)
-(*   column_round m; diagonal_round m; *)
-(*   column_round m; diagonal_round m; *)
-(*   column_round m; diagonal_round m; *)
-(*   column_round m; diagonal_round m; *)
-(*   column_round m; diagonal_round m; *)
-(*   column_round m; diagonal_round m *)
-
-(* private val chacha20_init:  *)
-(*   m:matrix -> k:key{disjoint m k} -> n:iv{disjoint m n} -> counter:u32 ->  *)
-(*   STL unit *)
-(*   (requires (fun h -> live h m /\ live h k /\ live h n )) *)
-(*   (ensures (fun h0 _ h1 -> live h1 m /\ modifies_1 m h0 h1)) *)
-
-(* private val fill: m:matrix -> i:u32 -> len:u32 {v i + v len <= 16}-> src:bytes {length src = 4 * v len} ->  *)
-(*   STL unit *)
-(*   (requires (fun h -> live h m /\ live h src /\ disjoint m src)) *)
-(*   (ensures (fun h0 _ h1 -> live h1 m /\ modifies_1 m h0 h1)) *)
-(* let rec fill m i len src = *)
-(*   if len <> 0ul then ( *)
-(*     m.(i) <- uint32_of_bytes (sub src 0ul 4ul);  *)
-(*     let len = len -^ 1ul in  *)
-(*     fill m (i +^ 1ul) len (sub src 4ul (4ul *^ len))) *)
-
-(* //review handling of endianness *)
-
-(* // RFC 7539 2.3 *)
-(* let chacha20_init m key iv counter = *)
-(*   m.(0ul) <- 0x61707865ul; *)
-(*   m.(1ul) <- 0x3320646eul; *)
-(*   m.(2ul) <- 0x79622d32ul; *)
-(*   m.(3ul) <- 0x6b206574ul; *)
-(*   fill m 4ul 8ul key; *)
-(*   m.(12ul) <- counter;  *)
-(*   fill m 13ul 3ul iv *)
-
-(* (\* lifted by hand for now: *\) *)
-(* private val add:  *)
-(*   m: matrix -> m0: matrix{disjoint m m0} ->  *)
-(*   i:u32 { i <^ 16ul } -> *)
-(*   STL unit *)
-(*   (requires (fun h -> live h m /\ live h m0)) *)
-(*   (ensures (fun h0 _ h1 -> live h1 m /\ modifies_1 m h0 h1)) *)
-(* let add m m0 i =  *)
-(*   m.(i) <- m.(i) +%^ m0.(i) *)
-
-(* private val sum_matrixes:  *)
-(*   m: matrix -> m0:matrix{disjoint m m0} ->  *)
-(*   STL unit *)
-(*   (requires (fun h -> live h m /\ live h m0)) *)
-(*   (ensures (fun h0 _ h1 -> live h1 m /\ modifies_1 m h0 h1)) *)
-(* let sum_matrixes m m0 = *)
-(* //let add i = upd m i (m.(i) +%^ m0.(i)) in // inlined?  *)
-(* // forUint32 0ul 15ul (fun i -> add m m0 i) *)
-(*   add m m0  0ul; *)
-(*   add m m0  1ul; *)
-(*   add m m0  2ul; *)
-(*   add m m0  3ul; *)
-(*   add m m0  4ul; *)
-(*   add m m0  5ul; *)
-(*   add m m0  6ul; *)
-(*   add m m0  7ul; *)
-(*   add m m0  8ul; *)
-(*   add m m0  9ul; *)
-(*   add m m0 10ul; *)
-(*   add m m0 11ul; *)
-(*   add m m0 12ul; *)
-(*   add m m0 13ul; *)
-(*   add m m0 14ul; *)
-(*   add m m0 15ul *)
-
-(* private val chacha20_update:  *)
-(*   output:bytes ->  *)
-(*   state:uint32s{length state = 32 /\ disjoint state output} -> *)
-(*   len:u32{v len <= 64 /\ length output >= v len} -> STL unit *)
-(*     (requires (fun h -> live h state /\ live h output)) *)
-(*     (ensures (fun h0 _ h1 -> live h1 output /\ live h1 state /\ modifies_2 output state h0 h1 )) *)
-(* let chacha20_update output state len = *)
-(*   (\* Initial state *\)  *)
-(*   let m  = sub state  0ul 16ul in *)
-(*   let m0 = sub state 16ul 16ul in // do we ever rely on m and m0 being contiguous? *)
-(*   blit m 0ul m0 0ul 16ul; *)
-(*   rounds m; *)
-(*   (\* Sum the matrixes *\) *)
-(*   sum_matrixes m m0; *)
-(*   (\* Serialize the state into byte stream *\) *)
-(*   bytes_of_uint32s output m len *)
-(* // avoid this copy when XORing? merge the sum_matrix and output loops? we don't use m0 afterward.  *)
-
-(* // computes one pseudo-random 64-byte block  *)
-(* // (consider fixing len to 64ul) *)
-
-(* val chacha20:  *)
-(*   output:bytes ->  *)
-(*   k:key -> *)
-(*   n:iv -> *)
-(*   counter: u32 -> *)
-(*   len:u32{v len <= v blocklen /\ v len <= length output} -> STL unit *)
-(*     (requires (fun h -> live h k /\ live h n /\ live h output)) *)
-(*     (ensures (fun h0 _ h1 -> live h1 output /\ modifies_1 output h0 h1 )) *)
-(* let chacha20 output key n counter len =  *)
-(*   push_frame (); *)
-(*   let state = create 0ul 32ul in *)
-(*   let m = sub state 0ul 16ul in *)
-(*   chacha20_init m key n counter; *)
-(*   chacha20_update output state len; *)
-(*   pop_frame () *)
-
-(* // Performance: it may be easier to precompute and re-use an expanded key (m0),  *)
-(* // to avoid passing around (key, counter, iv, constant), and only have m on the stack. *)
-(* // We may also merge the 3 final loops: sum_matrixes, bytes_of_uint32s, and outer XOR/ADD.  *)
-
-
-(* (\*** Counter-mode Encryption ***\) *)
-
-(* // The rest of this code is not specific to chacha20. *)
-(* // It is parameterized by the initial counter (0, or 1 for some AEAD) *)
-(* // and the block length (here 64 bytes). *)
-(* // It should appear after PRF idealization. *)
-
-(* private let prf = chacha20 *)
-
-(* // XOR-based encryption and decryption (just swap ciphertext and plaintext) *)
-(* val counter_mode:  *)
-(*   k:key -> n:iv -> counter:u32 ->  *)
-(*   len:u32{v counter + v len / v blocklen < pow2 32} -> *)
-(*   plaintext:bytes {length plaintext = v len /\ disjoint k plaintext} ->  *)
-(*   ciphertext:bytes {length ciphertext = v len /\ disjoint n ciphertext /\ disjoint k ciphertext /\ disjoint plaintext ciphertext} ->  *)
-(*   STL unit *)
-(*     (requires (fun h -> live h ciphertext /\ live h k /\ live h n /\ live h plaintext)) *)
-(*     (ensures (fun h0 _ h1 -> live h1 ciphertext /\ modifies_1 ciphertext h0 h1)) *)
-
-(* #reset-options "--z3timeout 100" *)
-(* // a bit slow, e.g. on the len precondition *)
-
-(* let rec counter_mode key iv counter len plaintext ciphertext = *)
-(*   if len =^ 0ul then ()  *)
-(*   else if len <^ blocklen  *)
-(*   then (\* encrypt final partial block *\) *)
-(*     begin *)
-(*       let cipher = sub ciphertext  0ul len in  *)
-(*       let plain  = sub plaintext   0ul len in  *)
-(*       prf cipher key iv counter len; *)
-(*       xor_bytes_inplace cipher plain len *)
-(*     end *)
-(*   else (\* encrypt full block *\) *)
-(*     begin *)
-(*       let cipher = sub ciphertext  0ul blocklen in *)
-(*       let plain  = sub plaintext   0ul blocklen in *)
-(*       prf cipher key iv counter blocklen; *)
-(*       xor_bytes_inplace cipher plain blocklen; *)
-(*       let len = len -^ blocklen in *)
-(*       let ciphertext = sub ciphertext blocklen len in *)
-(*       let plaintext  = sub plaintext  blocklen len in *)
-(*       counter_mode key iv (counter +^ 1ul) len plaintext ciphertext *)
-(*     end *)
-
+    chacha_encrypt_bytes_finish ctx m c rem)
